example/Dispatcher.thy
@@ -1,0 +1,817 @@
+theory Dispatcher
+
+imports
+  "../Parse"
+  "../Hoare/HoareTripleForBasicBlocks"
+  "./ToyExamplesBlocks"
+  "../Word_Lib/Word_Lemmas_32"
+begin
+
+definition 
+dispatch1_hash :: "32 word"
+where
+"dispatch1_hash == 0x3ecb5edf"
+
+definition 
+dispatch2_hash :: "32 word"
+where
+"dispatch2_hash == 0x8cd5b077"
+
+lemmas blocks_simps = build_blocks_def byteListInt_def find_block_def extract_indexes_def build_vertices_def
+ aux_basic_block.simps add_address_def block_pt_def
+
+value "parse_bytecode ''90''"
+
+value"blocks_list (build_blocks (parse_bytecode ''60606040526000357c0100000000000000000000000000000000000000000000000000000000900463ffffffff1680633ecb5edf1460475780638cd5b07714607b575b600080fd5b3415605157600080fd5b6065600480803590602001909190505060a1565b6040518082815260200191505060405180910390f35b3415608557600080fd5b608b60ad565b6040518082815260200191505060405180910390f35b6000600190505b919050565b6000600290505b905600a165627a7a72305820c9cf1e9d83721f6f9afecea62b7e868d98502ee8556dcaf6abb24acb8bc0d9fb0029''))"
+
+definition insts where
+"insts \<equiv>
+[Stack (PUSH_N [96]), Stack (PUSH_N [64]), Memory MSTORE, Stack (PUSH_N [0]), Stack CALLDATALOAD,
+  Stack (PUSH_N [1, 0, 0, 0, 0, 0, 0, 0, 0, 0, 0, 0, 0, 0, 0, 0, 0, 0, 0, 0, 0, 0, 0, 0, 0, 0, 0, 0, 0]),
+  Swap 0, Arith DIV, Stack (PUSH_N [255, 255, 255, 255]), Bits inst_AND, Dup 0,
+  Stack (PUSH_N [62, 203, 94, 223]), Arith inst_EQ, Stack (PUSH_N [71]), Pc JUMPI, Dup 0,
+  Stack (PUSH_N [140, 213, 176, 119]), Arith inst_EQ, Stack (PUSH_N [123]), Pc JUMPI, Pc JUMPDEST,
+  Stack (PUSH_N [0]), Dup 0, Unknown 253, Pc JUMPDEST, Info CALLVALUE, Arith ISZERO, Stack (PUSH_N [81]),
+  Pc JUMPI, Stack (PUSH_N [0]), Dup 0, Unknown 253, Pc JUMPDEST, Stack (PUSH_N [101]), Stack (PUSH_N [4]),
+  Dup 0, Dup 0, Stack CALLDATALOAD, Swap 0, Stack (PUSH_N [32]), Arith ADD, Swap 0, Swap 1, Swap 0, Stack POP,
+  Stack POP, Stack (PUSH_N [161]), Pc JUMP, Pc JUMPDEST, Stack (PUSH_N [64]), Memory MLOAD, Dup 0, Dup 2,
+  Dup 1, Memory MSTORE, Stack (PUSH_N [32]), Arith ADD, Swap 1, Stack POP, Stack POP, Stack (PUSH_N [64]),
+  Memory MLOAD, Dup 0, Swap 1, Arith SUB, Swap 0, Misc RETURN, Pc JUMPDEST, Info CALLVALUE, Arith ISZERO,
+  Stack (PUSH_N [133]), Pc JUMPI, Stack (PUSH_N [0]), Dup 0, Unknown 253, Pc JUMPDEST, Stack (PUSH_N [139]),
+  Stack (PUSH_N [173]), Pc JUMP, Pc JUMPDEST, Stack (PUSH_N [64]), Memory MLOAD, Dup 0, Dup 2, Dup 1,
+  Memory MSTORE, Stack (PUSH_N [32]), Arith ADD, Swap 1, Stack POP, Stack POP, Stack (PUSH_N [64]),
+  Memory MLOAD, Dup 0, Swap 1, Arith SUB, Swap 0, Misc RETURN, Pc JUMPDEST, Stack (PUSH_N [0]),
+  Stack (PUSH_N [1]), Swap 0, Stack POP, Pc JUMPDEST, Swap 1, Swap 0, Stack POP, Pc JUMP, Pc JUMPDEST,
+  Stack (PUSH_N [0]), Stack (PUSH_N [2]), Swap 0, Stack POP, Pc JUMPDEST, Swap 0, Pc JUMP, Misc STOP, Log LOG1,
+  Stack (PUSH_N [98, 122, 122, 114, 48, 88]), Arith SHA3, Unknown 201, Unknown 207, Unknown 30, Swap 13, Dup 3,
+  Stack (PUSH_N [31, 111, 154, 254, 206, 166, 43, 126, 134, 141, 152, 80, 46, 232, 85, 109, 202, 246, 171]),
+  Unknown 178, Unknown 74, Unknown 203, Dup 02, Unknown 192, Unknown 217, Unknown 251, Misc STOP, Unknown 41]"
+
+definition blocks where
+"blocks =
+\<lparr>blocks_indexes = [0, 56, 66, 71, 77, 81, 101, 123, 129, 133, 139, 161, 168, 173, 180, 183, 184, 226],
+    blocks_list = map_of [(0, [(0, Stack (PUSH_N [96])), (2, Stack (PUSH_N [64])), (4, Memory MSTORE), (5, Stack (PUSH_N [0])),
+            (7, Stack CALLDATALOAD),
+            (8, Stack (PUSH_N
+                        [1, 0, 0, 0, 0, 0, 0, 0, 0, 0, 0, 0, 0, 0, 0, 0, 0, 0, 0, 0, 0, 0, 0, 0, 0, 0, 0, 0,
+                         0])),
+            (38, Swap 0), (39, Arith DIV), (40, Stack (PUSH_N [255, 255, 255, 255])), (45, Bits inst_AND),
+            (46, Dup 0), (47, Stack (PUSH_N [62, 203, 94, 223])), (52, Arith inst_EQ),
+            (53, Stack (PUSH_N [71]))],
+        Jumpi),
+       (56, [(56, Dup 0), (57, Stack (PUSH_N [140, 213, 176, 119])), (62, Arith inst_EQ),
+             (63, Stack (PUSH_N [123]))],
+        Jumpi),
+       (66, [(66, Pc JUMPDEST), (67, Stack (PUSH_N [0])), (69, Dup 0), (70, Unknown 253)], No),
+       (71, [(71, Pc JUMPDEST), (72, Info CALLVALUE), (73, Arith ISZERO), (74, Stack (PUSH_N [81]))], Jumpi),
+       (77, [(77, Stack (PUSH_N [0])), (79, Dup 0), (80, Unknown 253)], No),
+       (81, [(81, Pc JUMPDEST), (82, Stack (PUSH_N [101])), (84, Stack (PUSH_N [4])), (86, Dup 0), (87, Dup 0),
+             (88, Stack CALLDATALOAD), (89, Swap 0), (90, Stack (PUSH_N [32])), (92, Arith ADD), (93, Swap 0),
+             (94, Swap 1), (95, Swap 0), (96, Stack POP), (97, Stack POP), (98, Stack (PUSH_N [161]))],
+        Jump),
+       (101, [(101, Pc JUMPDEST), (102, Stack (PUSH_N [64])), (104, Memory MLOAD), (105, Dup 0), (106, Dup 2),
+              (107, Dup 1), (108, Memory MSTORE), (109, Stack (PUSH_N [32])), (111, Arith ADD), (112, Swap 1),
+              (113, Stack POP), (114, Stack POP), (115, Stack (PUSH_N [64])), (117, Memory MLOAD),
+              (118, Dup 0), (119, Swap 1), (120, Arith SUB), (121, Swap 0), (122, Misc RETURN)],
+        No),
+       (123, [(123, Pc JUMPDEST), (124, Info CALLVALUE), (125, Arith ISZERO), (126, Stack (PUSH_N [133]))],
+        Jumpi),
+       (129, [(129, Stack (PUSH_N [0])), (131, Dup 0), (132, Unknown 253)], No),
+       (133, [(133, Pc JUMPDEST), (134, Stack (PUSH_N [139])), (136, Stack (PUSH_N [173]))], Jump),
+       (139, [(139, Pc JUMPDEST), (140, Stack (PUSH_N [64])), (142, Memory MLOAD), (143, Dup 0), (144, Dup 2),
+              (145, Dup 1), (146, Memory MSTORE), (147, Stack (PUSH_N [32])), (149, Arith ADD), (150, Swap 1),
+              (151, Stack POP), (152, Stack POP), (153, Stack (PUSH_N [64])), (155, Memory MLOAD),
+              (156, Dup 0), (157, Swap 1), (158, Arith SUB), (159, Swap 0), (160, Misc RETURN)],
+        No),
+       (161, [(161, Pc JUMPDEST), (162, Stack (PUSH_N [0])), (164, Stack (PUSH_N [1])), (166, Swap 0),
+              (167, Stack POP)],
+        Next),
+       (168, [(168, Pc JUMPDEST), (169, Swap 1), (170, Swap 0), (171, Stack POP)], Jump),
+       (173, [(173, Pc JUMPDEST), (174, Stack (PUSH_N [0])), (176, Stack (PUSH_N [2])), (178, Swap 0),
+              (179, Stack POP)],
+        Next),
+       (180, [(180, Pc JUMPDEST), (181, Swap 0)], Jump), (183, [(183, Misc STOP)], No),
+       (184, [(184, Log LOG1), (185, Stack (PUSH_N [98, 122, 122, 114, 48, 88])), (192, Arith SHA3),
+              (193, Unknown 201), (194, Unknown 207), (195, Unknown 30), (196, Swap 13), (197, Dup 3),
+              (198, Stack (PUSH_N
+                            [31, 111, 154, 254, 206, 166, 43, 126, 134, 141, 152, 80, 46, 232, 85, 109, 202,
+                             246, 171])),
+              (218, Unknown 178), (219, Unknown 74), (220, Unknown 203), (221, Dup 02), (222, Unknown 192),
+              (223, Unknown 217), (224, Unknown 251), (225, Misc STOP)],
+        No),
+       (226, [(226, Unknown 41)], No)],
+    all_blocks =
+      [(0, [(0, Stack (PUSH_N [96])), (2, Stack (PUSH_N [64])), (4, Memory MSTORE), (5, Stack (PUSH_N [0])),
+            (7, Stack CALLDATALOAD),
+            (8, Stack (PUSH_N
+                        [1, 0, 0, 0, 0, 0, 0, 0, 0, 0, 0, 0, 0, 0, 0, 0, 0, 0, 0, 0, 0, 0, 0, 0, 0, 0, 0, 0,
+                         0])),
+            (38, Swap 0), (39, Arith DIV), (40, Stack (PUSH_N [255, 255, 255, 255])), (45, Bits inst_AND),
+            (46, Dup 0), (47, Stack (PUSH_N [62, 203, 94, 223])), (52, Arith inst_EQ),
+            (53, Stack (PUSH_N [71]))],
+        Jumpi),
+       (56, [(56, Dup 0), (57, Stack (PUSH_N [140, 213, 176, 119])), (62, Arith inst_EQ),
+             (63, Stack (PUSH_N [123]))],
+        Jumpi),
+       (66, [(66, Pc JUMPDEST), (67, Stack (PUSH_N [0])), (69, Dup 0), (70, Unknown 253)], Next),
+       (71, [(71, Pc JUMPDEST), (72, Info CALLVALUE), (73, Arith ISZERO), (74, Stack (PUSH_N [81]))], Jumpi),
+       (77, [(77, Stack (PUSH_N [0])), (79, Dup 0), (80, Unknown 253)], Next),
+       (81, [(81, Pc JUMPDEST), (82, Stack (PUSH_N [101])), (84, Stack (PUSH_N [4])), (86, Dup 0), (87, Dup 0),
+             (88, Stack CALLDATALOAD), (89, Swap 0), (90, Stack (PUSH_N [32])), (92, Arith ADD), (93, Swap 0),
+             (94, Swap 1), (95, Swap 0), (96, Stack POP), (97, Stack POP), (98, Stack (PUSH_N [161]))],
+        Jump),
+       (101, [(101, Pc JUMPDEST), (102, Stack (PUSH_N [64])), (104, Memory MLOAD), (105, Dup 0), (106, Dup 2),
+              (107, Dup 1), (108, Memory MSTORE), (109, Stack (PUSH_N [32])), (111, Arith ADD), (112, Swap 1),
+              (113, Stack POP), (114, Stack POP), (115, Stack (PUSH_N [64])), (117, Memory MLOAD),
+              (118, Dup 0), (119, Swap 1), (120, Arith SUB), (121, Swap 0), (122, Misc RETURN)],
+        No),
+       (123, [(123, Pc JUMPDEST), (124, Info CALLVALUE), (125, Arith ISZERO), (126, Stack (PUSH_N [133]))],
+        Jumpi),
+       (129, [(129, Stack (PUSH_N [0])), (131, Dup 0), (132, Unknown 253)], Next),
+       (133, [(133, Pc JUMPDEST), (134, Stack (PUSH_N [139])), (136, Stack (PUSH_N [173]))], Jump),
+       (139, [(139, Pc JUMPDEST), (140, Stack (PUSH_N [64])), (142, Memory MLOAD), (143, Dup 0), (144, Dup 2),
+              (145, Dup 1), (146, Memory MSTORE), (147, Stack (PUSH_N [32])), (149, Arith ADD), (150, Swap 1),
+              (151, Stack POP), (152, Stack POP), (153, Stack (PUSH_N [64])), (155, Memory MLOAD),
+              (156, Dup 0), (157, Swap 1), (158, Arith SUB), (159, Swap 0), (160, Misc RETURN)],
+        No),
+       (161, [(161, Pc JUMPDEST), (162, Stack (PUSH_N [0])), (164, Stack (PUSH_N [1])), (166, Swap 0),
+              (167, Stack POP)],
+        Next),
+       (168, [(168, Pc JUMPDEST), (169, Swap 1), (170, Swap 0), (171, Stack POP)], Jump),
+       (173, [(173, Pc JUMPDEST), (174, Stack (PUSH_N [0])), (176, Stack (PUSH_N [2])), (178, Swap 0),
+              (179, Stack POP)],
+        Next),
+       (180, [(180, Pc JUMPDEST), (181, Swap 0)], Jump), (183, [(183, Misc STOP)], No),
+       (184, [(184, Log LOG1), (185, Stack (PUSH_N [98, 122, 122, 114, 48, 88])), (192, Arith SHA3),
+              (193, Unknown 201), (194, Unknown 207), (195, Unknown 30), (196, Swap 13), (197, Dup 3),
+              (198, Stack (PUSH_N
+                            [31, 111, 154, 254, 206, 166, 43, 126, 134, 141, 152, 80, 46, 232, 85, 109, 202,
+                             246, 171])),
+              (218, Unknown 178), (219, Unknown 74), (220, Unknown 203), (221, Dup 02), (222, Unknown 192),
+              (223, Unknown 217), (224, Unknown 251), (225, Misc STOP)],
+        No),
+       (226, [(226, Unknown 41)], Next)]\<rparr>"
+context
+notes if_split[ split del ] sep_fun_simps[simp del]
+gas_value_simps[simp add] pure_emp_simps[simp add]
+evm_fun_simps[simp add] sep_lc[simp del] sep_conj_first[simp add]
+pure_false_simps[simp add] iszero_stack_def[simp add]
+begin
+
+lemma aux1:
+"(word_of_int (bin_rcat 8 [62, 203, 94, 223]) ::w256)=
+    word_of_int (bin_rcat 8 [255, 255, 255, 255]) AND
+    (if word_of_int
+         (bin_rcat 8
+           [1, 0, 0, 0, 0, 0, 0, 0, 0, 0, 0, 0, 0, 0, 0, 0, 0, 0, 0,
+            0, 0, 0, 0, 0, 0, 0, 0, 0, 0]) =
+        (0::w256)
+     then word_of_int 0
+     else word_of_int
+           (uint
+             (read_word_from_bytes
+               (unat (word_of_int (bin_rcat 8 [0])))
+               (word_rsplit dispatch1_hash)) div
+            uint
+             (word_of_int
+               (bin_rcat 8
+                 [1, 0, 0, 0, 0, 0, 0, 0, 0, 0, 0, 0, 0, 0, 0, 0, 0,
+                  0, 0, 0, 0, 0, 0, 0, 0, 0, 0, 0, 0])::w256)))"
+apply(split if_splits)
+ apply(simp add: bin_rcat_def bin_cat_def)
+unfolding read_word_from_bytes_def dispatch1_hash_def
+apply simp
+apply (simp add: byte_list_fill_right_def)
+apply (simp add: word_rcat_def bin_rcat_def bin_cat_def  )
+done
+
+lemma stack_height_not_stack:
+"stack n m s \<Longrightarrow> \<not> stack_height h s"
+by(simp add: stack_height_def stack_def)
+
+lemma memory_elm_not_stack:
+"stack n m s \<Longrightarrow> \<not> memory8 h d s"
+by(simp add: memory8_def stack_def)
+
+lemma memory_range_not_stack:
+"stack n m s \<Longrightarrow> \<not> memory_range h d s"
+apply(induction d arbitrary: h s; simp add: stack_def)
+apply(simp add: memory8_sep)
+done
+
+lemma memory_not_stack:
+"stack n m s \<Longrightarrow> \<not> memory h d s"
+by(simp add: memory_def stack_def memory_range_not_stack)
+
+lemma gas_pred_not_stack:
+"stack n m s \<Longrightarrow> \<not> gas_pred h s"
+by(simp add: gas_pred_def stack_def)
+
+lemma continuing_not_stack:
+"stack n m s \<Longrightarrow> \<not> continuing s"
+by(simp add: continuing_def stack_def)
+
+lemma sent_data_not_stack:
+"stack n m s \<Longrightarrow> \<not> sent_data h s"
+by(simp add: sent_data_def stack_def)
+
+lemma sent_value_not_stack:
+"stack n m s \<Longrightarrow> \<not> sent_value h s"
+by(simp add: sent_value_def stack_def)
+
+lemma memory_usage_not_stack:
+"stack n m s \<Longrightarrow> \<not> memory_usage h s"
+by(simp add: memory_usage_def stack_def)
+
+lemma not_continuing_not_stack:
+"stack n m s \<Longrightarrow> \<not> not_continuing s"
+by(simp add: not_continuing_def stack_def)
+
+lemma program_counter_not_stack:
+"stack n m s \<Longrightarrow> \<not> program_counter p s"
+by(simp add: program_counter_def stack_def)
+
+lemma action_not_stack:
+"stack n m s \<Longrightarrow> \<not> action a s"
+by(simp add: action_def stack_def)
+
+lemmas not_stack =
+action_not_stack
+program_counter_not_stack
+not_continuing_not_stack
+memory_usage_not_stack
+sent_value_not_stack
+sent_data_not_stack
+continuing_not_stack
+gas_pred_not_stack
+memory_not_stack
+memory_range_not_stack
+stack_height_not_stack
+memory_elm_not_stack
+
+lemma stack_height_first:
+"(a \<and>* stack_height h \<and>* b) = (stack_height h \<and>* a \<and>* b)"
+by(rule sep.mult.left_commute)
+
+lemma stack_first:
+"\<forall>n m s. stack n m s \<longrightarrow> \<not> a s \<Longrightarrow>
+(a \<and>* stack h d \<and>* b) = (stack h d \<and>* a \<and>* b)"
+by(rule sep.mult.left_commute)
+
+method order_sep_conj=
+(simp add: stack_first not_stack)?,
+(simp add: stack_height_first)?
+
+method sep_imp_solve =
+(clarsimp?),
+(rule conjI),
+  (clarsimp simp add: word_rcat_simps)?,
+  order_sep_conj?,
+  (sep_cancel, simp?)+,
+  (erule instantiate_emp)?,
+(simp add:word_rcat_simps)?
+value "word_rsplit (0x3ecb5edf::32 word):: byte list"
+find_theorems "size" name:word
+
+lemma length_word_rsplit_32:
+"length (word_rsplit (x::w256)::byte list) = 32"
+by(simp add: length_word_rsplit_exp_size' word_size)
+
+lemma word_of_int_hash_not_0:
+"word_of_int
+ (bin_rcat 8
+   [1, 0, 0, 0, 0, 0, 0, 0, 0, 0, 0, 0, 0, 0, 0, 0, 0, 0,
+    0, 0, 0, 0, 0, 0, 0, 0, 0, 0, 0]) \<noteq>
+(0::w256)"
+by(simp add: bin_rcat_def bin_cat_def)
+
+
+lemmas calldataload_simps=
+read_word_from_bytes_def
+byte_list_fill_right_def
+
+lemmas words_simps=
+word_of_int_hash_not_0
+word_rcat_eq
+length_word_rsplit_32
+
+method blocks_rule_vcg=
+rule blocks_jumpi_uint |
+rule blocks_jump_uint |
+rule blocks_next |
+rule blocks_no
+
+method block_vcg=
+((blocks_rule_vcg; (rule refl)?), triple_seq_vcg),
+(sep_imp_solve; simp?)+,
+(simp_all add: word_rcat_simps bin_cat_def)
+
+context
+notes
+  words_simps[simp add]
+  calldataload_simps[simp add]
+  M_def[simp add]
+  Cmem_def[simp add]
+  memory_range.simps[simp del]
+begin
+
+lemma spec_fun1:
+"\<exists>r.
+triple 
+  (
+program_counter 0 ** stack_height 0 ** (sent_data (word_rsplit (0x3ecb5edf::32 word))) ** sent_value 0 **
+   memory_usage 0 ** continuing ** gas_pred 3000 ** memory (word_rcat [64::byte]) (word_rcat [x::byte]::256 word) **
+   memory (word_rcat [96::byte]) (word_rcat [y::byte]::256 word))
+  blocks
+  (action (ContractReturn (word_rsplit (1:: w256))) ** r)"
+apply (simp add: blocks_def triple_def)
+apply(rule exI)
+apply(block_vcg)
+apply(block_vcg)
+apply(block_vcg)
+apply(block_vcg)
+apply(block_vcg)
+apply(block_vcg)
+apply(sep_cancel)+
+done
+
+lemma spec_fun2:
+"\<exists>r.
+triple 
+  (
+program_counter 0 ** stack_height 0 ** (sent_data (word_rsplit (0x8cd5b077::32 word))) ** sent_value 0 **
+   memory_usage 0 ** continuing ** gas_pred 3000 ** memory (word_rcat [64::byte]) (word_rcat [x::byte]::256 word) **
+   memory (word_rcat [96::byte]) (word_rcat [y::byte]::256 word))
+  blocks
+  (action (ContractReturn (word_rsplit (2:: w256))) ** r)"
+apply (simp add: blocks_def triple_def)
+apply(rule exI)
+apply(block_vcg)
+apply(block_vcg)
+apply(block_vcg)
+apply(block_vcg)
+	apply(block_vcg)
+	apply(block_vcg)+
+apply(sep_cancel)+
+done
+
+lemma length_word_rsplit_4:
+"length (word_rsplit (x::32 word)::byte list) = 4"
+by(simp add: length_word_rsplit_exp_size' word_size)
+
+
+lemma power_mult:
+"((\<lambda>s. s * (x::int)) ^^ m) = (\<lambda>s. s * (x ^ m))"
+apply(rule ext)
+apply(induction m; simp)
+done
+
+lemma div_mult2_eq_word:
+"unat b * unat d < 2 ^ len_of TYPE('a) \<Longrightarrow>
+(a:: 'a :: len word) div (b * d) = a div b div d"
+  apply unat_arith
+  apply clarsimp
+  apply (subst unat_mult_lem [THEN iffD1], simp)
+  apply(rule div_mult2_eq)
+done
+
+lemma word_mult_left_cancel: 
+  "(0 :: 'a :: len word) < y \<Longrightarrow> unat x * unat y < 2 ^ len_of TYPE('a) \<Longrightarrow>
+   unat z * unat y < 2 ^ len_of TYPE('a) \<Longrightarrow>
+    (x * y = z * y) = (x = z)"
+  apply unat_arith
+  apply clarsimp
+  apply(rule iffI)
+   defer
+   apply(simp)
+  apply(drule unat_cong)
+  apply (subst (asm)unat_mult_lem [THEN iffD1], simp)
+  apply(simp)
+  apply (subst (asm)unat_mult_lem [THEN iffD1], simp)
+  apply auto
+  done
+
+lemma word_rcat_div_1_a_not0:
+"a \<noteq> 0 \<Longrightarrow>
+ n \<le> 27 \<Longrightarrow>
+ m \<le> 27 \<Longrightarrow>
+16777216 * uint a + 65536 * uint b + 256 * uint d + uint e = f \<Longrightarrow>
+((word_rcat ([a::byte,b,d,e] @ replicate (Suc n) 0))::w256) div
+(word_rcat ([1::byte] @ (replicate (Suc m) 0))::w256) =
+(word_rcat ([a,b,d,e] @ (replicate n 0))::w256) div
+(word_rcat ([1::byte] @ (replicate m 0))::w256)"
+apply(simp add: word_rcat_def bin_rcat_def bin_cat_num)
+apply(rule subst[OF mult.commute])
+apply(simp add: foldl_conv_fold power_mult)
+apply(subst Word.word_ubin.norm_Rep[where x=a, simplified])+
+apply(subst Word.word_ubin.norm_Rep[where x=b, simplified])+
+apply(subst Word.word_ubin.norm_Rep[where x=d, simplified])+
+apply(subst Word.word_ubin.norm_Rep[where x=e, simplified])+
+apply(rule subst[OF wi_hom_mult, where P="\<lambda>x. x div _ = _"])
+apply(rule subst[OF wi_hom_mult[where b=256 and a="16777216 * uint a + 65536 * uint b + 256 * uint d + uint e", simplified], where P="\<lambda>x. x * _ div _ = _"])
+apply(rule subst[OF wi_hom_mult, where P="\<lambda>x. _ div x = _"])
+apply(rule subst[OF wi_hom_mult, where P="\<lambda>x. _ = x div _"])
+apply(simp add: mult.commute)
+apply(subst div_mult2_eq_word)
+ apply(simp add: unat_def uint_word_of_int)
+ apply(subst nat_mono_iff[where z="2^248", simplified])
+ apply(subst int_mod_eq')
+   apply(simp)
+  apply(rule Power.linordered_semidom_class.power_strict_increasing[where N=32 and a=256, simplified])
+  apply(simp)
+ apply(rule Power.linordered_semidom_class.power_strict_increasing[where N=31 and a=256, simplified])
+ apply(simp)
+apply(simp add: mult.assoc mult.commute[where a="0x100"])
+apply(simp add: sym[OF mult.assoc])
+apply(subst Word.word_div_mult)
+  apply(simp_all)
+apply(subgoal_tac "f > 0")
+ apply(simp add: unat_def)
+ apply(subst nat_mono_iff[where z="2^248", simplified])
+ apply(subst wi_hom_mult)
+ apply(subst sym[OF word_less_alt[where a="word_of_int (f * 256^n)" and b="word_of_int (uint (2^248::w256))::w256", simplified]])
+ apply(subst wi_less[where n="f * 256^n" and m="uint (2^248::w256)" and 'a=256, simplified])
+ apply(subgoal_tac "f < 256 ^4"; simp)
+	apply(subst int_mod_eq'[where a="f * 256 ^ n" and b="2^256", simplified]; simp?)
+   apply(rule mult_strict_mono[where d="256^28::int" and b=4294967296, simplified]; simp?)
+   apply(rule Power.linordered_semidom_class.power_strict_increasing[where N=28 and a=256, simplified], simp)
+  apply(rule mult_less_le_imp_less[where d="256^27::int" and b=4294967296, simplified]; simp?)
+  apply(rule Power.linordered_semidom_class.power_increasing[where N=27 and a=256, simplified], simp)
+ apply(drule sym; simp)
+ apply(insert uint_lt[where w="a"])[1]
+ apply(insert uint_lt[where w="b"])[1]
+ apply(insert uint_lt[where w="d"])[1]
+ apply(insert uint_lt[where w="e"])[1]
+ apply(simp)
+apply(drule sym; simp)
+apply(subgoal_tac "uint a > 0")
+ apply(insert uint_0[where w=b])[1]
+ apply(insert uint_0[where w=d])[1]
+ apply(insert uint_0[where w=e])[1]
+ apply(arith)
+apply(insert uint_0[where w=a])[1]
+apply(subgoal_tac "uint a \<noteq> 0")
+ apply(arith)
+apply(rule notI)
+apply(simp add: uint_0_iff)
+done
+
+method word32_not_0_aux=
+		 (subgoal_tac "uint a > 0"),
+	  (arith),
+	 (subgoal_tac "uint a \<noteq> 0"),
+	  (arith),
+	 (rule notI),
+	 (simp add: uint_0_iff)
+
+lemma word32_not_0:
+	"\<And>a b d e.(a \<noteq> 0 \<or> b\<noteq>0 \<or> d\<noteq>0 \<or> e\<noteq>0) \<Longrightarrow> (uint a * 16777216 + uint b * 65536 + uint d * 256 + uint e) > 0"
+apply(cut_tac w=a in uint_0)
+apply(cut_tac w=b in uint_0)
+apply(cut_tac w=d in uint_0)
+apply(cut_tac w=e in uint_0)
+	apply(erule disjE, word32_not_0_aux)
+	apply(erule disjE)
+		apply(rename_tac b a d e, word32_not_0_aux)
+	apply(erule disjE)
+		apply(rename_tac d b a e, word32_not_0_aux)
+	apply(rename_tac e b d a, word32_not_0_aux)
+done
+	
+lemma word_rcat_div_1:
+"a \<noteq> 0 \<or> b\<noteq>0 \<or> d\<noteq>0 \<or> e\<noteq>0 \<Longrightarrow>
+ n \<le> 27 \<Longrightarrow>
+ m \<le> 27 \<Longrightarrow>
+16777216 * uint a + 65536 * uint b + 256 * uint d + uint e = f \<Longrightarrow>
+((word_rcat ([a::byte,b,d,e] @ replicate (Suc n) 0))::w256) div
+(word_rcat ([1::byte] @ (replicate (Suc m) 0))::w256) =
+(word_rcat ([a,b,d,e] @ (replicate n 0))::w256) div
+(word_rcat ([1::byte] @ (replicate m 0))::w256)"
+apply(simp add: word_rcat_def bin_rcat_def bin_cat_num)
+apply(rule subst[OF mult.commute])
+apply(simp add: foldl_conv_fold power_mult)
+apply(subst Word.word_ubin.norm_Rep[where x=a, simplified])+
+apply(subst Word.word_ubin.norm_Rep[where x=b, simplified])+
+apply(subst Word.word_ubin.norm_Rep[where x=d, simplified])+
+apply(subst Word.word_ubin.norm_Rep[where x=e, simplified])+
+apply(rule subst[OF wi_hom_mult, where P="\<lambda>x. x div _ = _"])
+apply(rule subst[OF wi_hom_mult[where b=256 and a="16777216 * uint a + 65536 * uint b + 256 * uint d + uint e", simplified], where P="\<lambda>x. x * _ div _ = _"])
+apply(rule subst[OF wi_hom_mult, where P="\<lambda>x. _ div x = _"])
+apply(rule subst[OF wi_hom_mult, where P="\<lambda>x. _ = x div _"])
+apply(simp add: mult.commute)
+apply(subst div_mult2_eq_word)
+ apply(simp add: unat_def uint_word_of_int)
+ apply(subst nat_mono_iff[where z="2^248", simplified])
+ apply(subst int_mod_eq')
+   apply(simp)
+  apply(rule Power.linordered_semidom_class.power_strict_increasing[where N=32 and a=256, simplified])
+  apply(simp)
+ apply(rule Power.linordered_semidom_class.power_strict_increasing[where N=31 and a=256, simplified])
+ apply(simp)
+apply(simp add: mult.assoc mult.commute[where a="0x100"])
+apply(simp add: sym[OF mult.assoc])
+apply(subst Word.word_div_mult)
+  apply(simp_all)
+apply(subgoal_tac "f > 0")
+ apply(simp add: unat_def)
+ apply(subst nat_mono_iff[where z="2^248", simplified])
+ apply(subst wi_hom_mult)
+ apply(subst sym[OF word_less_alt[where a="word_of_int (f * 256^n)" and b="word_of_int (uint (2^248::w256))::w256", simplified]])
+ apply(subst wi_less[where n="f * 256^n" and m="uint (2^248::w256)" and 'a=256, simplified])
+ apply(subgoal_tac "f < 256 ^4"; simp)
+	apply(subst int_mod_eq'[where a="f * 256 ^ n" and b="2^256", simplified]; simp?)
+   apply(rule mult_strict_mono[where d="256^28::int" and b=4294967296, simplified]; simp?)
+   apply(rule Power.linordered_semidom_class.power_strict_increasing[where N=28 and a=256, simplified], simp)
+  apply(rule mult_less_le_imp_less[where d="256^27::int" and b=4294967296, simplified]; simp?)
+  apply(rule Power.linordered_semidom_class.power_increasing[where N=27 and a=256, simplified], simp)
+ apply(drule sym; simp)
+ apply(insert uint_lt[where w="a"])[1]
+ apply(insert uint_lt[where w="b"])[1]
+ apply(insert uint_lt[where w="d"])[1]
+ apply(insert uint_lt[where w="e"])[1]
+ apply(simp)
+apply(drule sym; simp add: mult.commute)
+apply(rule word32_not_0[simplified], assumption)
+done
+
+lemma word_rcat_div1:
+"a \<noteq> 0 \<or> b\<noteq>0 \<or> d\<noteq>0 \<or> e\<noteq>0 \<Longrightarrow>
+ n \<le> 28 \<Longrightarrow>
+16777216 * uint a + 65536 * uint b + 256 * uint d + uint e = f \<Longrightarrow>
+((word_rcat ([a::byte,b,d,e] @ replicate n 0))::w256) div
+(word_rcat ([1::byte] @ (replicate n 0))::w256) =
+(word_rcat ([a,b,d,e])::w256)"
+apply(induction n; simp)
+ apply(subgoal_tac "word_rcat [1::byte] = (1::(w256))")
+  apply(simp add: word_div_def)
+ apply(simp add: word_rcat_simps)
+apply(subst word_rcat_div_1[simplified]; simp)
+done
+
+definition bit_mask :: "32 word \<Rightarrow> 256 word" where
+"bit_mask z =  4294967295 AND
+    word_of_int
+     (uint
+       (word_rcat
+         (word_rsplit z @
+          [0::byte, 0, 0, 0, 0, 0, 0, 0, 0, 0, 0, 0, 0, 0, 0, 0, 0, 0, 0, 0,
+           0, 0, 0, 0, 0, 0, 0, 0])::w256) div
+      26959946667150639794667015087019630673637144422540572481103610249216)"
+find_theorems word_rsplit
+lemma
+	"z \<noteq> 0 \<Longrightarrow>
+	 word_rsplit (z::32 word) = [a, b, d, e::byte] \<Longrightarrow>
+	 a \<noteq> 0 \<or> b \<noteq> 0 \<or> d \<noteq> 0 \<or> e \<noteq> 0"
+	apply(simp add: word_rsplit_def)
+		apply(simp add: bin_rsplit_def bin_last_def bin_rest_def)
+	oops
+	value "(2^32::32word)"
+lemma word_rsplit_upt:
+  "\<lbrakk> size x = len_of TYPE('a :: len) * n; n \<noteq> 0 \<rbrakk>
+    \<Longrightarrow> word_rsplit x = map (\<lambda>i. ucast (x >> i * len_of TYPE ('a)) :: 'a word) (rev [0 ..< n])"
+sorry
+lemma w:
+ "  word_rsplit w = sw \<Longrightarrow>
+  \<forall>k m. k < length sw \<longrightarrow> m < size (hd sw) \<longrightarrow>
+  rev sw ! k !! m = w !! (k * size (hd sw) + m)"
+apply (clarsimp)
+apply (rule test_bit_rsplit[OF sym, rule_format] ; simp)
+done
+
+lemma list0_x:
+"\<forall>k<Suc (Suc (Suc (Suc 0))).
+       \<forall>m<8.
+          [0, 0, 0, 0::byte] ! k !! m = z !! (k * 8 + m) \<Longrightarrow>
+n <32 \<Longrightarrow>
+    \<not> z !! n"
+apply(drule_tac x="n div 8" in spec)
+apply(drule mp)
+apply unat_arith
+apply(drule_tac x="n mod 8" in spec)
+ apply(drule mp, arith)
+apply(simp)
+apply(subgoal_tac "[0, 0, 0, 0] ! (n div 8) = (0::byte)")
+apply(simp)
+apply(subgoal_tac "n div 8 < 4")
+apply (subst nth_Cons', clarsimp  split: if_split)+
+apply (unat_arith)
+done
+
+lemma word_rsplit_0':
+	"word_rsplit (z::32 word) = [0,0,0,0::byte] \<Longrightarrow>
+	z =0"
+apply (drule w)
+apply clarsimp
+apply (simp add: word_size)
+apply (word_bitwise)
+apply ((rule conjI)?, erule list0_x, simp)+
+done
+
+lemma "(x::32 word) AND y = y AND x"
+oops
+
+value "(0xffffffff::256 word) !! 32"
+
+lemma
+"n < 256 \<Longrightarrow> n \<ge> (8* length zs) \<Longrightarrow>  \<not>(word_rcat (zs::byte list)::w256) !! n"
+apply(induction zs arbitrary: n)
+ apply(simp add: word_rcat_simps )
+apply(simp add: word_rcat_def)
+apply(simp add: bin_rcat_def)
+sorry
+
+lemma word_rcat_nul_bits:
+"n \<ge> 32 \<Longrightarrow>  \<not>((word_rcat ([a,b,d,e]::byte list))::w256) !! n"
+apply(simp add: word_rcat_def)
+apply(simp add: bin_rcat_def)
+apply(simp add: bin_cat_def)
+apply(simp add: bintrunc_def)
+done
+
+lemma word_rsplit_32:
+"\<exists>a b d e. word_rsplit (z::32 word) = [a,b,d,e::byte]"
+apply(insert length_word_rsplit_4[where x=z])
+apply(case_tac "word_rsplit z::byte list")
+ apply(simp)
+apply(rename_tac list, case_tac list, simp)
+apply(rename_tac list, case_tac list, simp)
+apply(rename_tac list, case_tac list, simp)
+  apply(simp)
+done
+
+lemma word_rcat_rsplit_ucast:
+"(word_rcat (word_rsplit z::byte list)::w256) = ucast (z::32 word)"
+ apply(simp add: ucast_def)
+ apply (rule word_eqI)
+ apply(case_tac "n < 32")
+  apply (clarsimp simp add : test_bit_rcat word_size)
+  apply (subst refl [THEN test_bit_rsplit])
+    apply (simp_all add: word_size 
+      refl [THEN length_word_rsplit_size [simplified not_less [symmetric], simplified]])
+  apply safe
+     apply(subst (asm) word_test_bit_def, assumption)
+    apply(arith)
+   apply(subst word_test_bit_def, assumption)
+  apply(drule leI)
+  apply(insert word_rsplit_32[where z=z], clarsimp)[1]
+  apply(drule_tac a=a and b=b and d=d and e=e in word_rcat_nul_bits, simp)
+ apply(drule leI)
+ apply(drule bin_nth_uint_imp, simp)
+done
+
+lemma word_rcat_bits_eq:
+"n < 32 \<Longrightarrow>  ((word_rcat (word_rsplit z::byte list))::w256) !! n = (z::32 word) !! n"
+apply(insert word_rsplit_32[where z=z])
+apply(clarsimp)
+apply(simp add: word_rcat_def)
+apply(simp add: bin_rcat_def)
+apply(simp add: bin_cat_def)
+apply(simp add: bintrunc_def)
+oops
+
+lemma word_rcat_rsplit_max: "(word_rcat [a,b,d,e::byte]::w256) \<le> mask 32"
+apply(subst le_mask_iff)
+  apply (rule word_eqI)
+ apply (subst nth_shiftr)
+ apply(simp add: word_size)
+ apply(rule word_rcat_nul_bits)
+apply(simp)
+done
+
+lemma
+	eval_bit_mask':
+	"bit_mask z = word_rcat (word_rsplit (z::32 word)::byte list)"
+	apply(simp add: bit_mask_def)
+  apply(subgoal_tac "\<exists>a b d e. word_rsplit (z::32 word) = [a::byte,b,d,e]")
+	apply(rule subst[OF uint_div[where x="word_rcat
+         (word_rsplit z @
+          [0, 0, 0, 0, 0, 0, 0, 0, 0, 0, 0, 0, 0, 0,
+           0, 0, 0, 0, 0, 0, 0, 0, 0, 0, 0, 0, 0,
+           0])" and y="26959946667150639794667015087019630673637144422540572481103610249216::w256", simplified],
+          where P="\<lambda>x. _ AND word_of_int x = _"])
+  apply(case_tac "z\<noteq>0")
+  apply(clarsimp)
+   apply(cut_tac a=a and b=b and d=d and e=e and n=28 in word_rcat_div1)
+   apply(subgoal_tac "\<not>([a::byte,b,d,e] = [0,0,0,0::byte])")
+    apply(simp)
+   apply(rule notI)
+    apply(drule sym[where s="word_rsplit _"]; simp)
+    apply(drule word_rsplit_0')
+   apply(simp)+
+   apply(subgoal_tac "word_rcat [1::byte, 0, 0, 0, 0, 0, 0, 0, 0, 0, 0, 0, 0, 0, 0, 0, 0, 0, 0, 0, 0, 0, 0, 0, 0, 0, 0, 0, 0] =
+        (0x100000000000000000000000000000000000000000000000000000000::w256)")
+    apply(clarsimp)
+   (* apply(thin_tac _, thin_tac _,thin_tac _, thin_tac _) *)
+   apply(thin_tac "word_rcat _ = _", thin_tac " _ = word_rcat _")
+   apply (subgoal_tac "0xFFFFFFFF = (mask 32::256 word)")
+   apply(simp only:word_bw_comms)
+ apply (subst word_bw_comms(1))
+   apply (subst le_mask_imp_and_mask)
+   apply(rule word_rcat_rsplit_max)
+apply(simp)
+apply(simp add: mask_def)
+apply(thin_tac _)+
+apply(simp add: word_rcat_simps bin_cat_def)
+apply(clarsimp)
+apply(subst (asm) Word_Lemmas_32.word_rsplit_0)
+apply(clarsimp simp add: word_rcat_simps bin_cat_def)
+apply(rule word_rsplit_32)
+done
+
+lemma
+	eval_bit_mask:
+	"bit_mask z = ucast (z::32 word)"
+apply(subst eval_bit_mask')
+apply(subst word_rcat_rsplit_ucast)
+apply(rule refl)
+done
+
+
+lemma bit_mask_noteq:
+"x \<noteq> y \<Longrightarrow> bit_mask x \<noteq> bit_mask y"
+apply(rule notI)
+apply(subst (asm) eval_bit_mask)+
+apply(drule up_ucast_inj; simp)
+done
+
+method bit_mask_solve=
+(insert length_word_rsplit_4[where x=z])[1],
+(split if_split_asm; simp)+,
+(drule bit_mask_noteq),
+(subst (asm) eval_bit_mask)+,
+(simp add: ucast_def)
+
+lemmas bit_mask_rev = sym[OF bit_mask_def]
+
+lemma spec_fail:
+notes
+  bit_mask_rev[simp add]
+shows
+"z \<noteq> dispatch1_hash \<Longrightarrow>
+z \<noteq> dispatch2_hash \<Longrightarrow>
+\<exists>r.
+triple 
+  (
+program_counter 0 ** stack_height 0 ** (sent_data (word_rsplit (z::32 word)::byte list)) ** sent_value 0 **
+   memory_usage 0 ** continuing ** gas_pred 3000 ** memory (word_rcat [64::byte]) (word_rcat [x::byte]::256 word) **
+   memory (word_rcat [96::byte]) (word_rcat [y::byte]::256 word))
+  blocks
+  (action (ContractFail [ShouldNotHappen]) ** r)"
+apply (simp add: blocks_def triple_def dispatch1_hash_def dispatch2_hash_def)
+apply(rule exI)
+apply(block_vcg; bit_mask_solve)
+apply(block_vcg; bit_mask_solve)
+apply(block_vcg)
+apply(sep_cancel)+
+done
+
+definition return_action' ::"32 word \<Rightarrow> contract_action" where
+"return_action' z = 
+  (if z = dispatch1_hash then ContractReturn (word_rsplit (1:: w256))
+  else (if z = dispatch2_hash then ContractReturn (word_rsplit (2:: w256))
+  else ContractFail [ShouldNotHappen]))"
+
+
+lemma verify_dispatcher:
+"\<exists>r.
+triple 
+  (
+program_counter 0 ** stack_height 0 ** (sent_data (word_rsplit (z::32 word)::byte list)) ** sent_value 0 **
+   memory_usage 0 ** continuing ** gas_pred 3000 ** memory (word_rcat [64::byte]) (word_rcat [x::byte]::256 word) **
+   memory (word_rcat [96::byte]) (word_rcat [y::byte]::256 word))
+  blocks
+  (action (return_action' z) ** r)"
+apply(simp add: return_action'_def)
+apply(case_tac "z = dispatch1_hash")
+ apply(simp add: spec_fun1[simplified] dispatch1_hash_def dispatch2_hash_def return_action'_def)
+apply(case_tac "z = dispatch2_hash")
+ apply(simp add: dispatch1_hash_def dispatch2_hash_def return_action'_def)
+ apply(rule spec_fun2[simplified])
+apply(simp add: spec_fail return_action'_def)
+done
+
+definition return_action:: "(32 word \<Rightarrow> contract_action option) \<Rightarrow> 32 word \<Rightarrow> contract_action" where
+"return_action m w = (case m w of 
+   None \<Rightarrow> ContractFail [ShouldNotHappen]
+ | Some a \<Rightarrow> a)"
+
+lemma unspec_contract:
+"(z = dispatch1_hash \<longrightarrow> triple_blocks blocks (program_counter 71 \<and>* restx) (71, the (blocks_list blocks 71)) (action xx \<and>* restbx)) \<Longrightarrow>
+(z = dispatch2_hash \<longrightarrow> triple_blocks blocks (program_counter 123 \<and>* resty) (123, the (blocks_list blocks 123)) (action yy \<and>* restby)) \<Longrightarrow> 
+\<exists>rest. 
+ triple
+  (program_counter 0 ** stack_height 0 ** (sent_data (word_rsplit (z::32 word)::byte list)) ** sent_value 0 **
+   memory_usage 0 ** continuing ** gas_pred 3000 ** memory (word_rcat [64::byte]) (word_rcat [m64::byte]::256 word) **
+   memory (word_rcat [96::byte]) (word_rcat [m96::byte]::256 word))
+  blocks
+  (action (return_action (map_of [(dispatch1_hash, xx), (dispatch2_hash, yy)]) z) \<and>* rest) "
+apply (simp add: dispatch1_hash_def dispatch2_hash_def)
+apply(rule exI)
+apply(subst blocks_def, simp add: triple_def)
+apply(block_vcg)
+apply(case_tac "z=dispatch1_hash")
+ apply(simp add: dispatch1_hash_def word_rcat_simps bin_cat_def)
+oops
+
+end
+end
